concur/ThreadLinkingBack.v
@@ -4,7 +4,7 @@ Require Import Smallstep SmallstepClosed.
 Require Import ValueAnalysis.
 Require Import MultiLibs CMulti AsmMulti.
 Require Import Extends InjectFootprint CA.
-Require Import CallconvBig Ext Injp CAnew Composition.
+Require Import CallconvBig HCompBig Ext Injp CAnew Composition.
 Require Import ThreadLinking.
 
 Section ConcurSim.
@@ -3317,22 +3317,6 @@ Section ConcurSim.
 
        
   End BSIM.
-
-  Definition final_noundef (lts : semantics li_c li_c) : Prop :=
-   forall s v m se,
-        Smallstep.final_state (lts se) s (cr v m) ->
-        v <> Vundef.
-    
-  Definition after_external_receptive (lts : semantics li_c li_c) : Prop :=
-    forall s q r se,
-      Smallstep.at_external (lts se) s q ->
-      exists s', Smallstep.after_external (lts se) s r s'.
-
-  Definition initial_state_receptive (lts : semantics li_c li_c) : Prop :=
-    forall s vf sg args se m m',
-      Smallstep.initial_state (lts se) (cq vf sg args m) s ->
-      Mem.sup_include (Mem.support m) (Mem.support m') ->
-      exists s', Smallstep.initial_state (lts se) (cq vf sg args m') s'.
 
   Lemma BSIM : GS.backward_simulation cc_compcert OpenC OpenA ->
                determinate_big OpenC ->
