cdemo/Demoproof.v
@@ -16,7 +16,7 @@ Require Import Encrypt EncryptSpec Encryptproof.
 Require Import Client Server.
 
 Require Import SmallstepLinking VCompBig HCompBig CallConvLibs.
-Require Import Composition CMulti AsmMulti ThreadLinking Compiler.
+Require Import Composition Clight Asm CMulti AsmMulti ThreadLinking ThreadLinkingBack Compiler.
 
 
 Import GS.
@@ -82,5 +82,93 @@ Section LINKING.
   Proof.
     apply Opensim_to_Globalsim; eauto. apply module_linking_correct.
   Qed.
+
+  Lemma c_spec_receptive : receptive c_spec.
+  Proof.
+    unfold compose in compose_c2. unfold option_map in compose_c2.
+    destruct link in compose_c2; inv compose_c2.
+    eapply HCompBig.semantics_receptive. intros. destruct i.
+    eapply Clight.semantics_receptive.
+    unfold compose in compose_c1. unfold option_map in compose_c1.
+    destruct link in compose_c1; inv compose_c1.
+    eapply HCompBig.semantics_receptive. intros. destruct i.
+    { red. intros. constructor.
+      intros. inv H. eexists. simpl. inv H0. econstructor; eauto.
+      red. intros. inv H. simpl. lia. }
+    eapply Clight.semantics_receptive.
+  Qed.
+                     
+  
+  Lemma c_spec_determinate_big : determinate_big c_spec.
+  Admitted.
+
+  Lemma compose_after_receptive : forall (Lc1 Lc2 Lc : Smallstep.semantics li_c li_c),
+      compose Lc1 Lc2 = Some Lc ->
+      after_external_receptive Lc1 ->
+      after_external_receptive Lc2 ->
+      after_external_receptive Lc.
+  Proof.
+    intros Lc1 Lc2 Lc Hc Hr1 Hr2.
+    unfold compose in Hc. unfold option_map in Hc.
+    destruct link in Hc; inv Hc.
+    red. intros. inv H. destruct i.
+    - red in Hr1.
+      exploit Hr1; eauto. instantiate (1:= r).
+      intros [s' Hy].
+      eexists. econstructor; eauto.
+    - exploit Hr2; eauto. instantiate (1:= r).
+      intros [s' Hy]. eexists. econstructor; eauto.
+  Qed.
+
+  Lemma compose_initial_receptive : forall (Lc1 Lc2 Lc : Smallstep.semantics li_c li_c),
+      compose Lc1 Lc2 = Some Lc ->
+      initial_state_receptive Lc1 ->
+      initial_state_receptive Lc2 ->
+      initial_state_receptive Lc.
+  Proof.
+    intros Lc1 Lc2 Lc Hc Hi1 Hi2.
+    unfold compose in Hc. unfold option_map in Hc.
+    destruct link in Hc; inv Hc.
+    red. intros. inv H. destruct i.
+    - exploit Hi1; eauto.
+      intros [s' Hi].
+      eexists. econstructor. instantiate (1:=true). simpl.
+      eauto.
+    - exploit Hr2; eauto. instantiate (1:= r).
+      intros [s' Hy]. eexists. econstructor; eauto.
+  Admitted.
+  
+  Lemma c_spec_receptive_after_external : after_external_receptive c_spec.
+  Proof.
+    eapply compose_after_receptive; eauto.
+    eapply Clight_after_external_receptive.
+    eapply compose_after_receptive; eauto.
+    red. intros. inv H.
+    eapply Clight_after_external_receptive.
+  Qed.
+
+  Lemma c_spec_receptive_initial_state : initial_state_receptive c_spec.
+    eapply compose_initial_receptive. eauto.
+    apply Clight_initial_state_receptive.
+    eapply compose_initial_receptive. eauto.
+    red. intros. inv H. eexists. econstructor; eauto.
+    apply Clight_initial_state_receptive.
+  Qed.
+  
+  Theorem module_linking_back :
+    backward_simulation cc_compcert c_spec (Asm.semantics asm_prog).
+  Proof.
+    eapply GS.forward_to_backward_simulation. eapply module_linking_correct.
+    apply c_spec_receptive.
+    eapply Asm.semantics_determinate.
+  Qed.
+
+  Theorem thread_linking_back :
+    Closed.backward_simulation (Concur_sem_c c_spec) (Concur_sem_asm (Asm.semantics asm_prog)).
+    apply BSIM; eauto. eapply module_linking_back.
+    apply c_spec_determinate_big.
+    apply c_spec_receptive_after_external.
+    apply c_spec_receptive_initial_state.
+  Qed.     
 
 End LINKING.
